repair resource exchange example

src/examples/lib/excl_ops.v
@@ -1,14 +1,14 @@
 From Equations Require Import Equations.
 From iris.algebra Require Import gmap_view.
 From iris_named_props Require Import named_props.
-From nextgen Require Import cmra_morphism_extra gmap_view_transformation.
-From self.nextgen Require Import hvec nextgen_promises.
+From nextgen Require Import cmra_morphism_extra.
+From self.nextgen Require Import hvec nextgen_promises gmap_view_transformation.
 From iris.proofmode Require Import proofmode.
 
 Set Default Proof Using "Type*".
 
 (* TODO: upstream this tactic. *)
-Definition drop_word s := substring (1 + findex 0 " " s) (String.length s) s.
+Definition drop_word s := String.substring (1 + String.findex 0 " " s) (String.length s) s.
 
 Tactic Notation "iPickedInAgree" constr(Hs) :=
   let na := eval vm_compute in (drop_word Hs) in
@@ -16,33 +16,32 @@ Tactic Notation "iPickedInAgree" constr(Hs) :=
   iClear na.
 
 (* The exclusive ghost resource: [gset_disj nat]. *)
-Definition excl_opsR : cmra := gmap_viewR nat unitO.
+Definition excl_opsR : cmra := gmap_viewUR nat (agreeR unitO).
 Class excl_opsG (Σ: gFunctors) (Ω: gGenCmras Σ) := {
   excl_ops_inG :: genInDepsG Σ Ω excl_opsR [#];
 }.
 Section Ghosts.
   Context `{!excl_opsG Σ Ω}.
 
-  Definition drop_op (p: nat) n (_: unit): option _ :=
+  Definition drop_op (p: nat) n (_: unitO): option unitO :=
     if decide (n < p) then Some () else None.
 
   #[global] Instance drop_op_maptrans p: MapTrans (drop_op p).
   Proof.
-    split; last solve_proper.
-    intros. done.
+    split; last solve_proper; intros; done.
   Qed.
   
   Definition excl_ops_trans (p: nat): excl_opsR → excl_opsR :=
-    map_entry_lift_gmap_view (drop_op p).
+    (map_entry_lift_gmap_view (V := unitO) (drop_op p)).
 
   Definition excl_ops_pred (p: nat): pred_over excl_opsR :=
     λ t, ∃ p', p ≤ p' ∧ t = excl_ops_trans p'.
   
   Definition ops_auth γ (n: nat): iProp Σ :=
-    gen_own γ (gmap_view_auth (DfracOwn 1) (map_seq 0 (repeat () n))).
+    gen_own γ (gmap_view_auth (DfracOwn 1) (to_agree <$> map_seq 0 (repeat () n))).
 
   Definition ops_frag γ (n: nat): iProp Σ :=
-    "frag" ∷ gen_own γ (gmap_view_frag n (DfracOwn 1) ()) ∗
+    "frag" ∷ gen_own γ (gmap_view_frag n (DfracOwn 1) (to_agree ())) ∗
     "#frag_rely_self" ∷ ∃ p', ⌜ n < p' ⌝ ∗ rely_self γ (excl_ops_pred p').
 
   Definition ops_token γ (p: nat) :=
@@ -110,13 +109,15 @@ Section Ghosts.
   Qed.
   
   Lemma ops_auth_grow {γ n}:
-    ops_auth γ n ==∗ ops_auth γ (S n) ∗ gen_own γ (gmap_view_frag n (DfracOwn 1) ()).
+    ops_auth γ n ==∗ ops_auth γ (S n) ∗ gen_own γ (gmap_view_frag n (DfracOwn 1) (to_agree ())).
   Proof.
     iIntros "ops_auth".
     iMod (gen_own_update with "ops_auth") as "[$ $]"; last done.
-    rewrite map_seq_grow.
-    apply gmap_view_alloc; last done.
-    rewrite lookup_map_seq_0 lookup_ge_None repeat_length //.
+    rewrite map_seq_grow fmap_insert.
+    apply: (gmap_view_alloc _ _ (DfracOwn 1) (to_agree ())); try done.
+    rewrite lookup_fmap lookup_map_seq_0.
+    apply fmap_None.
+    rewrite lookup_ge_None repeat_length //.
   Qed.
     
   Lemma ops_auth_ops_frag_false {γ} n:
@@ -125,11 +126,15 @@ Section Ghosts.
     False.
   Proof.
     iIntros "auth". iNamed 1.
-    iDestruct (gen_own_valid_2 with "auth frag") as %[_ contra]%gmap_view_both_valid_L.
-    rewrite lookup_map_seq_0 in contra.
-    apply lookup_lt_Some in contra.
-    rewrite repeat_length in contra.
-    lia.
+    iDestruct (gen_own_valid_2 with "auth frag") as %[_ [_ contra]]%gmap_view_both_valid.
+    rewrite lookup_fmap lookup_map_seq_0 in contra.
+    destruct (repeat () n !! n) eqn:Heq; rewrite Heq /= in contra.
+    - apply lookup_lt_Some in Heq.
+      rewrite repeat_length in Heq.
+      lia.
+    - symmetry in contra.
+      rewrite None_equiv_eq in contra.
+      done.
   Qed.
 
   Lemma ops_token_strengthen {γ p} p':
@@ -149,14 +154,6 @@ Section Ghosts.
     iDestruct (token_to_rely with "token") as "#rely".
     iDestruct (rely_to_rely_self with "rely") as "$".
     done.
-  Qed.
-
-  Lemma map_entry_lift_gmap_view_auth dq (m: gmap nat unit) map_entry :
-    (map_entry_lift_gmap_view map_entry (gmap_view_auth dq m)) =
-    (gmap_view_auth dq (map_imap map_entry m)).
-  Proof.
-    unfold map_entry_lift_gmap_view, fmap_view, fmap_pair. simpl.
-    rewrite agree_map_to_agree. done.
   Qed.
 End Ghosts.
 Opaque ops_frag.
